Remove bin_op_eval and rename bin_op_eval2 to bin_op_eval.
Renamed SSA to Instruction.

SSA.v
@@ -9,20 +9,23 @@ Local Open Scope type_scope.
 This is the definition of a SSA language.
 A program is a list of SSA instructions.
 The label of an instruction is its position in the list.
-There is arithmetic instructions, and non conditionals and conditionals
+There is arithmetic instructions, conditionals and non conditionals
 branching instructions.
 *)
 
 Definition variable := string.
+
 Definition label := nat.
 
 (* Every variable has a value, even the non defined ones *)
 Definition RegisterMap := total_map Z.
+
 (* The label is the program counter *)
 Definition state := RegisterMap * label.
 
 Local Open Scope string_scope.
 Local Open Scope list_scope.
+Local Open Scope Z_scope.
 
 (* Basics binary arithmetic opcodes *)
 Inductive BinArithOpCode :=
@@ -30,17 +33,8 @@ Inductive BinArithOpCode :=
 | OpMul
 | OpLe.
 
-Local Open Scope Z_scope.
-
 (* The evaluation of a binary operation *)
-Definition bin_op_eval (R : RegisterMap) (op : BinArithOpCode) (v1 v2 : variable) :=
-  match op with
-  | OpAdd => (eval_map R v1) + (eval_map R v2)
-  | OpMul => (eval_map R v1) * (eval_map R v2)
-  | OpLe => if (eval_map R v1) <=? (eval_map R v2) then 1 else 0
-  end.
-
-Definition bin_op_eval2 (op : BinArithOpCode) (v1 v2 : Z) :=
+Definition bin_op_eval (op : BinArithOpCode) (v1 v2 : Z) :=
   match op with
   | OpAdd => v1 + v2
   | OpMul => v1 * v2
@@ -48,15 +42,16 @@ Definition bin_op_eval2 (op : BinArithOpCode) (v1 v2 : Z) :=
   end.
 
 (* An SSA instruction *)
-Inductive SSA :=
+Inductive Instruction :=
 | Const (v: variable) (c: Z)
-| BinOp (v: variable) (b: BinArithOpCode) (op1 op2: variable): v <> op1 -> v <> op2 -> SSA
+| BinOp (v: variable) (b: BinArithOpCode) (op1 op2: variable): v <> op1 -> v <> op2 -> Instruction
 | Br (l: label) (params: list (variable * variable))
-| BrC (c: variable) (l1: label) (params1: list (variable * variable)) (l2: label) (params2: list (variable * variable)).
+| BrC (c: variable) (l1: label) (params1: list (variable * variable))
+      (l2: label) (params2: list (variable * variable)).
 
 (* An SSA program *)
 Definition Program :=
-  list SSA.
+  list Instruction.
 
 Fixpoint affect_variables (R: RegisterMap) (vars: list (variable * variable)) :=
   match vars with
@@ -65,10 +60,10 @@ Fixpoint affect_variables (R: RegisterMap) (vars: list (variable * variable)) :=
   end.
 
 (* Do one step given an instruction *)
-Definition ssa_step (inst : SSA) (R : RegisterMap) (l : label) :=
+Definition ssa_step (inst : Instruction) (R : RegisterMap) (l : label) :=
   match inst with
-  | Const v x => (v !-> x; R , Nat.add l 1)
-  | BinOp v op x1 x2 _ _ => (v !-> bin_op_eval R op x1 x2 ; R, Nat.add l 1)
+  | Const v x => (v !-> x; R, Nat.add l 1)
+  | BinOp v op x1 x2 _ _ => (v !-> bin_op_eval op (eval_map R x1) (eval_map R x2) ; R, Nat.add l 1)
   | Br l' params => (affect_variables R params, l')
   | BrC c l1 params1 l2 params2 =>
     if eval_map R c =? 0 then
@@ -81,7 +76,7 @@ Local Open Scope nat_scope.
 
 (* Small step semantics *)
 Inductive step : Program -> state -> state -> Prop :=
-| SingleStep (p: Program) (R R': RegisterMap) (l l': label) (s: SSA):
+| SingleStep (p: Program) (R R': RegisterMap) (l l': label) (s: Instruction):
     l < List.length p ->
     l' < List.length p ->
     Some s = List.nth_error p l ->
